Refactoring arrays to use sigma and omicron

Sem.v
@@ -45,8 +45,7 @@ Inductive tm : Set :=
   | tm_load  : tm   -> tm
   | tm_asg   : tm   -> tm -> tm
   | tm_acq   : tm   -> tm -> tm
-  | tm_cr    : addr -> tm -> tm       (* critical region  *)
-  | tm_ptm   : option nat -> tm -> tm (* protected term   *)
+  | tm_cr    : addr -> tm -> tm (* critical region *)
   (* concurrency *)
   | tm_spawn : tm -> tm
   .
@@ -95,7 +94,6 @@ Notation "t1 ':=' t2"     := (tm_asg t1 t2)       (in custom elo_tm at level 70,
                                                               no associativity).
 Notation "'acq' t1 t2"    := (tm_acq t1 t2)       (in custom elo_tm at level 0).
 Notation "'cr' t1 t2"     := (tm_cr t1 t2)        (in custom elo_tm at level 0).
-Notation "'ptm' tid t"    := (tm_ptm tid t)       (in custom elo_tm at level 0).
 Notation "'spawn' t"      := (tm_spawn t)         (in custom elo_tm at level 0).
 
 Reserved Notation "Gamma '|--' t 'is' T" (at level 40).
@@ -124,7 +122,6 @@ Inductive value : tm -> Prop :=
   | v_num  : forall n, value <{nat n}>
   | v_fun  : forall x Tx t, value <{fn x Tx t}> 
   | v_ref  : forall ad T, value <{&ad : T}>
-  | v_ptm  : forall ad t, value <{ptm ad t}>
   .
 
 (* ------------------------------------------------------------------------- *)
@@ -142,19 +139,32 @@ Inductive eff : Set :=
   .
 
 (* ------------------------------------------------------------------------- *)
+(* cells                                                                     *)
+(* ------------------------------------------------------------------------- *)
+
+Inductive cell : Type :=
+  | cell_triple (t : tm) (T : ty) (otid : option nat)
+  .
+
+Notation "'(' t ',' T ',' otid ')'" := (cell_triple t T otid).
+
+Notation " c '.t' " := (let (t, _, _) := c in t) (at level 9).
+Notation " c '.T' " := (let (_, T, _) := c in T) (at level 9).
+Notation " c '.X' " := (let (_, _, X) := c in X) (at level 9).
+
+(* ------------------------------------------------------------------------- *)
 (* aliases                                                                   *)
 (* ------------------------------------------------------------------------- *)
 
-Definition ctx := map ty.
-
-Definition mem     := list (tm * ty).
+Definition ctx     := map ty.
+Definition mem     := list cell.
 Definition threads := list tm.
 Definition trace   := list (nat * eff).
 
-Definition tm_default  := <{unit}>.
-Definition ty_default  := `Unit`.
-Definition mem_default := (tm_default, ty_default).
-Definition tc_default  := (0, e_none).
+Definition tm_default   := <{unit}>.
+Definition ty_default   := `Unit`.
+Definition cell_default := (tm_default, ty_default, None).
+Definition tc_default   := (0, e_none).
 
 (* ------------------------------------------------------------------------- *)
 (* typing                                                                    *)
@@ -231,10 +241,6 @@ Inductive type_of : ctx -> tm -> ty -> Prop :=
     empty |-- t is T ->
     Gamma |-- <{cr ad t}> is T
 
-  | T_ptm : forall Gamma tid t T,
-    empty |-- t is T ->
-    Gamma |-- <{ptm tid t}> is T
-
   | T_spawn : forall Gamma t T,
     safe Gamma |-- t is T ->
     Gamma |-- <{spawn t}> is `Unit` 
@@ -262,7 +268,6 @@ Fixpoint subst (x : id) (tx t : tm) : tm :=
   | <{t1 := t2   }> => <{([x := tx] t1) := ([x := tx] t2)}>
   | <{acq t1 t2  }> => <{acq ([x := tx] t1) ([x := tx] t2)}>
   | <{cr ad t'   }> => <{cr ad ([x := tx] t')}> (* could it be "t"? *)
-  | <{ptm _ _    }> => t
   (* concurrency *)
   | <{spawn t'   }> => <{spawn ([x := tx] t')}>
   end
@@ -292,17 +297,9 @@ Inductive tstep : tm -> eff -> tm -> Prop :=
     t --[e]--> t' ->
     <{new t : T}> --[e]--> <{new t' : T}>
 
-  | ts_newR : forall ad t T,
+  | ts_new : forall ad t T,
     value t ->
-    <{new t : r&T}>  --[e_alloc ad t `r&T`]--> <{&ad : r&T}>
-
-  | ts_newX : forall ad t T,
-    value t ->
-    <{new t : x&T}> --[e_alloc ad <{ptm None t}> `x&T`]--> <{&ad : x&T}>
-
-  | ts_newW : forall ad t T,
-    value t ->
-    <{new t : w&T}> --[e_alloc ad t `w&T`]--> <{&ad : w&T}>
+    <{new t : T}> --[e_alloc ad t T]--> <{&ad : T}>
 
   (* Load *)
   | ts_load1 : forall t t' e,
@@ -358,55 +355,66 @@ Inductive tstep : tm -> eff -> tm -> Prop :=
 (* operational semantics -- memory step                                      *)
 (* ------------------------------------------------------------------------- *)
 
-Notation " ths '[' tid ']' " := (ths[tid] or tm_default)
-  (at level 9, tid at next level).
-
-Notation " m '[' ad '].tm' " := (fst (m[ad] or mem_default))
+Notation " m '[' ad '].cell' " := (m[ad] or cell_default)
   (at level 9, ad at next level).
 
-Notation " m '[' ad '].ty' " := (snd (m[ad] or mem_default))
+Notation " m '[' ad '].t' " := ((m[ad] or cell_default).t)
+  (at level 9, ad at next level).
+
+Notation " m '[' ad '].T' " := ((m[ad] or cell_default).T)
+  (at level 9, ad at next level).
+
+Notation " m '[' ad '].X' " := ((m[ad] or cell_default).X)
+  (at level 9, ad at next level).
+
+Notation " m '[' ad '.tT' '<-' t T ']' " :=
+  (m[ad <- (t, T, m[ad].cell.X)])
+  (at level 9, ad at next level, t at next level).
+
+Notation " m '[' ad '.X' '<-' X ']' " :=
+  (m[ad <- (m[ad].cell.t, m[ad].cell.T, X)])
   (at level 9, ad at next level).
 
 Inductive mstep : mem -> tm -> eff -> mem -> tm -> Prop :=
-  | ms_none : forall m t t',
-    t --[e_none]--> t' ->
-    m / t ==[e_none]==> m / t'
+  | ms_none : forall m t1 t2,
+    t1 --[e_none]--> t2 ->
+    m / t1 ==[e_none]==> m / t2
 
-  | ms_alloc : forall m t t' ad te T,
+  | ms_alloc : forall m t1 t2 ad t T,
     ad = #m ->
-    t --[e_alloc ad te T]--> t' ->
-    m / t ==[e_alloc ad te T]==> (m +++ (te, T)) / t'
+    t1 --[e_alloc ad t T]--> t2 ->
+    m / t1 ==[e_alloc ad t T]==> (m +++ (t, T, None)) / t2
 
-  | ms_read : forall m t t' ad te,
+  | ms_read : forall m t1 t2 ad,
     ad < #m ->
-    te = m[ad].tm ->
-    t --[e_read ad te]--> t' ->
-    m / t ==[e_read ad te]==> m / t'
+    t1 --[e_read ad m[ad].t]--> t2 ->
+    m / t1 ==[e_read ad m[ad].t]==> m / t2
 
-  | ms_write : forall m t t' ad te T,
+  | ms_write : forall m t1 t2 ad t T,
     ad < #m ->
-    t --[e_write ad te T]--> t' ->
-    m / t ==[e_write ad te T]==> m[ad <- (te, T)] / t'
+    t1 --[e_write ad t T]--> t2 ->
+    m / t1 ==[e_write ad t T]==> m[ad.tT <- t T] / t2
 
-  | ms_acq : forall m t t' tid ad te T,
+  | ms_acq : forall m t1 t2 tid ad,
     ad < #m ->
-    m[ad].tm = <{ptm None te}> ->
-    m[ad].ty = T ->
-    t --[e_acq tid ad te]--> t' ->
-    m / t ==[e_acq tid ad te]==> m[ad <- (tm_ptm (Some tid) te, T)] / t'
+    m[ad].X = None ->
+    t1 --[e_acq tid ad m[ad].t]--> t2 ->
+    m / t1 ==[e_acq tid ad m[ad].t]==> m[ad.X <- Some tid] / t2
 
-  | ms_rel : forall m t t' te tid ad T,
+  | ms_rel : forall m t1 t2 tid ad,
     ad < #m ->
-    m[ad].tm = tm_ptm (Some tid) te ->
-    m[ad].ty = T ->
-    t --[e_rel tid ad]--> t' ->
-    m / t ==[e_rel tid ad]==> m[ad <- (<{ptm None te}>, T)] / t'
+    m[ad].X = Some tid->
+    t1 --[e_rel tid ad]--> t2 ->
+    m / t1 ==[e_rel tid ad]==> m[ad.X <- None] / t2
 
   where "m / t '==[' e ']==>' m' / t'" := (mstep m t e m' t').
 
 (* ------------------------------------------------------------------------- *)
 (* operational semantics -- step                                             *)
 (* ------------------------------------------------------------------------- *)
+
+Notation " ths '[' tid ']' " := (ths[tid] or tm_default)
+  (at level 9, tid at next level).
 
 Inductive cstep : mem -> threads -> nat -> eff -> mem -> threads -> Prop :=
   | cs_mem : forall m m' t' ths tid e,
