ValidReferences.v
@@ -1,5 +1,8 @@
 From Elo Require Import Core.
 
+From Elo Require Import Preservation_.
+From Elo Require Import WellTypedTerm.
+From Elo Require Import ValidPointerTypes.
 From Elo Require Import ValidAddresses.
 
 (* ------------------------------------------------------------------------- *)
@@ -26,15 +29,15 @@ Inductive valid_references (m : mem) : tm -> Prop :=
     valid_references m <{call t1 t2}> 
 
   | vr_refR : forall T ad,
-    m[ad].ty = `r&T` ->
+    m[ad].T = `r&T` ->
     valid_references m <{&ad : r&T}>
 
   | vr_refX : forall T ad,
-    m[ad].ty = `x&T` ->
+    m[ad].T = `x&T` ->
     valid_references m <{&ad : x&T}>
 
   | vr_refW : forall T ad,
-    m[ad].ty = `w&T` ->
+    m[ad].T = `w&T` ->
     valid_references m <{&ad : w&T}>
 
   | vr_new : forall T t,
@@ -59,10 +62,6 @@ Inductive valid_references (m : mem) : tm -> Prop :=
     valid_references m t ->
     valid_references m <{cr ad t}>
 
-  | vr_ptm : forall tid t,
-    valid_references m t ->
-    valid_references m <{ptm tid t}>
-
   | vr_spawn : forall t,
     valid_references m t ->
     valid_references m <{spawn t}>
@@ -83,7 +82,6 @@ Local Ltac _vr tt :=
   | H : valid_references _ <{_ := _   }> |- _ => tt H
   | H : valid_references _ <{acq _ _  }> |- _ => tt H
   | H : valid_references _ <{cr _ _   }> |- _ => tt H
-  | H : valid_references _ <{ptm _ _  }> |- _ => tt H
   | H : valid_references _ <{spawn _  }> |- _ => tt H
   end.
 
@@ -110,22 +108,19 @@ Proof.
   intros. ind_tstep; inv_vr; eauto.
 Qed.
 
-(*
 Local Lemma vr_write_effect : forall m t1 t2 ad t T,
   well_typed_term t1 ->
   valid_references m t1 ->
   (* --- *)
   t1 --[e_write ad t T]--> t2 ->
-  exists Tm, T = `w&Tm`
-          /\ empty |-- t is Tm
-          /\ empty |-- m[ad].tm is Tm
-          /\ m[ad].ty = `w&Tm`.
+  T = m[ad].T.
 Proof.
   intros * [T' ?] **. generalize dependent T'.
-  ind_tstep; intros; inv_typeof; inv_vr; eauto.
-  inv_typeof. inv_vr. eauto.
+  ind_tstep; intros; invc_typeof; invc_vr; eauto.
+  invc_typeof. invc_vr. eauto.
 Qed.
 
+(*
 Local Lemma vr_rel_effect : forall m t1 t2 otid ad,
   well_typed_term t1 ->
   valid_references m t1 ->
@@ -164,60 +159,32 @@ Proof.
   induction t; eauto using valid_references;
   inv_vad; inv_vr; eauto using valid_references;
   (eapply vr_refR || eapply vr_refX || eapply vr_refW);
-  simpl_array; assumption.
+  sigma; assumption.
 Qed.
 
-Lemma vr_mem_setX : forall m t te ad T,
+Lemma vr_mem_setW : forall m t ad te Te,
   ad < #m ->
-  empty |-- te is T ->
-  m[ad].ty = `x&T` ->
+  Te = m[ad].T ->
   (* --- *)
   valid_references m t ->
-  valid_references m[ad <- (te, `x&T`)] t.
+  valid_references m[ad.tT <- te Te] t.
 Proof.
   intros.
-  induction t; eauto using valid_references;
-  invc_vr; eauto using valid_references;
+  induction t; try invc_vr; eauto using valid_references;
   (eapply vr_refR || eapply vr_refX || eapply vr_refW);
-  Array.sgs; trivial;
-  match goal with H1 : _[?ad1].ty = _, H2 : _[?ad2].ty = _ |- _ =>
-    rewrite H1 in H2; inv H2
-  end;
-  trivial.
+  omicron; eauto.
 Qed.
 
-Lemma vr_mem_setW : forall m t te ad T,
+Lemma vr_mem_setX : forall m t ad X,
   ad < #m ->
-  empty |-- te is T ->
-  m[ad].ty = `w&T` ->
   (* --- *)
   valid_references m t ->
-  valid_references m[ad <- (te, `w&T`)] t.
+  valid_references m[ad.X <- X] t.
 Proof.
   intros.
-  induction t; eauto using valid_references;
-  invc_vr; eauto using valid_references;
+  induction t; try invc_vr; eauto using valid_references;
   (eapply vr_refR || eapply vr_refX || eapply vr_refW);
-  Array.sgs; trivial;
-  match goal with H1 : _[?ad1].ty = _, H2 : _[?ad2].ty = _ |- _ =>
-    rewrite H1 in H2; inv H2
-  end;
-  trivial.
-Qed.
-
-Local Lemma vr_mem_ptm : forall m otid1 otid2 ad t T,
-  ad < #m ->
-  empty |-- t is T ->
-  m[ad].ty = `x&T` ->
-  (* --- *)
-  forall_memory m (valid_references m) ->
-  m[ad].tm = <{ptm otid1 t}> ->
-  valid_references m[ad <- (<{ptm otid2 t}>, `x&T`)] t.
-Proof.
-  intros * ? ? ? H Hptm.
-  specialize (H ad). simpl in H.
-  rewrite Hptm in H. invc_vr.
-  eauto using type_of, vr_mem_setX.
+  omicron; eauto.
 Qed.
 
 (* none -------------------------------------------------------------------- *)
@@ -234,7 +201,7 @@ Qed.
 
 (* alloc ------------------------------------------------------------------- *)
 
-Lemma vr_preservation_mem_alloc : forall m t1 t2 t T,
+Lemma vr_preservation_mem_alloc : forall m t1 t2 t T X,
   well_typed_term t1 ->
   forall_memory m (valid_addresses m) ->
   valid_addresses m t1 ->
@@ -242,35 +209,34 @@ Lemma vr_preservation_mem_alloc : forall m t1 t2 t T,
   (* --- *)
   forall_memory m (valid_references m) ->
   t1 --[e_alloc (#m) t T]--> t2 ->
-  forall_memory (m +++ (t, T)) (valid_references (m +++ (t, T))).
+  forall_memory (m +++ (t, T, X)) (valid_references (m +++ (t, T, X))).
 Proof.
-  intros ** ad.
-  decompose sum (lt_eq_lt_dec ad (#m)); subst; simpl_array;
+  intros ** ad. omicron;
   eauto using vr_mem_add, valid_references; (* optimization *)
   eauto using vr_mem_add, vr_tstep_alloc_term.
 Qed.
 
-Lemma vr_preservation_alloc : forall m t1 t2 t T,
+Lemma vr_preservation_alloc : forall m t1 t2 t T X,
   well_typed_term t1 ->
   valid_addresses m t1 ->
   (* --- *)
   valid_references m t1 ->
   t1 --[e_alloc (#m) t T]--> t2 ->
-  valid_references (m +++ (t, T)) t2.
+  valid_references (m +++ (t, T, X)) t2.
 Proof.
   intros * [T ?] **. generalize dependent T.
   ind_tstep; intros; inv_vr; inv_typeof; inv_vad;
   eauto using vr_mem_add, valid_references;
   (eapply vr_refR || eapply vr_refX || eapply vr_refW);
-  simpl_array; eauto using type_of, empty_eq_safe_empty.
+  sigma; eauto using type_of, empty_eq_safe_empty.
 Qed.
 
-Lemma vr_preservation_unt_alloc : forall m t1 t2 tu ad t T,
+Lemma vr_preservation_unt_alloc : forall m t1 t2 tu ad t T X,
   valid_addresses m tu ->
   (* --- *)
   valid_references m tu ->
   t1 --[e_alloc ad t T]--> t2 ->
-  valid_references (m +++ (t, T)) tu.
+  valid_references (m +++ (t, T, X)) tu.
 Proof.
   intros.
   ind_tstep; eauto using vr_mem_add, valid_references.
@@ -279,10 +245,10 @@ Qed.
 (* read -------------------------------------------------------------------- *)
 
 Lemma vr_preservation_read : forall m t1 t2 ad,
-  valid_references m m[ad].tm ->
+  valid_references m m[ad].t ->
   (* --- *)
   valid_references m t1 ->
-  t1 --[e_read ad m[ad].tm]--> t2 ->
+  t1 --[e_read ad m[ad].t]--> t2 ->
   valid_references m t2.
 Proof.
   intros.
@@ -298,16 +264,10 @@ Lemma vr_preservation_mem_write : forall m t1 t2 ad t T,
   ad < #m ->
   forall_memory m (valid_references m) ->
   t1 --[e_write ad t T]--> t2 ->
-  forall_memory m[ad <- (t, T)] (valid_references m[ad <- (t, T)]).
+  forall_memory m[ad.tT <- t T] (valid_references m[ad.tT <- t T]).
 Proof.
   intros ** ?.
-  assert (Hctwe : exists Tm, T = `w&Tm`
-    /\ empty |-- t is Tm
-    /\ empty |-- m[ad].tm is Tm
-    /\ m[ad].ty = `w&Tm`)
-    by eauto using vr_write_effect.
-  decompose record Hctwe; subst.
-  Array.sgs; eauto using vr_mem_setW, vr_tstep_write_term.
+  omicron; eauto using vr_mem_setW, vr_tstep_write_term, vr_write_effect.
 Qed.
 
 Lemma vr_preservation_write : forall m t1 t2 ad t T,
@@ -316,17 +276,11 @@ Lemma vr_preservation_write : forall m t1 t2 ad t T,
   ad < #m ->
   valid_references m t1 ->
   t1 --[e_write ad t T]--> t2 ->
-  valid_references (m[ad <- (t, T)]) t2.
+  valid_references (m[ad.tT <- t T]) t2.
 Proof.
   intros.
-  assert (Hctwe : exists Tm, T = `w&Tm`
-    /\ empty |-- t is Tm
-    /\ empty |-- m[ad].tm is Tm
-    /\ m[ad].ty = `w&Tm`)
-    by eauto using vr_write_effect.
-  decompose record Hctwe; subst.
-  ind_tstep; intros; invc_wtt; invc_vr;
-  eauto using vr_mem_setW, valid_references.
+  ind_tstep; invc_wtt; invc_vr;
+  eauto using vr_mem_setW, vr_write_effect, valid_references.
 Qed.
 
 Lemma vr_preservation_unt_write : forall m t1 t2 tu ad t T,
@@ -336,79 +290,81 @@ Lemma vr_preservation_unt_write : forall m t1 t2 tu ad t T,
   ad < #m ->
   valid_references m tu ->
   t1 --[e_write ad t T]--> t2 ->
-  valid_references m[ad <- (t, T)] tu.
+  valid_references m[ad.tT <- t T] tu.
 Proof.
   intros.
-  assert (Hctwe : exists Tm, T = `w&Tm`
-    /\ empty |-- t is Tm
-    /\ empty |-- m[ad].tm is Tm
-    /\ m[ad].ty = `w&Tm`)
-    by eauto using vr_write_effect.
-  decompose record Hctwe; subst.
-  eauto using vr_mem_setW.
+  eauto using vr_mem_setW, vr_write_effect.
 Qed.
 
 (* acq --------------------------------------------------------------------- *)
 
-(* TODO *)
+Lemma vr_preservation_mem_acq : forall m t1 t2 tid ad t X,
+  forall_memory m well_typed_term ->
+  well_typed_term t1 ->
+  valid_references m t1 ->
+  (* --- *)
+  ad < #m ->
+  forall_memory m (valid_references m) ->
+  t1 --[e_acq tid ad t]--> t2 ->
+  forall_memory m[ad.X <- X] (valid_references m[ad.X <- X]).
+Proof.
+  intros ** ?. omicron; eauto using vr_mem_setX.
+Qed.
+
+Lemma vr_preservation_acq : forall m t1 t2 tid ad X,
+  forall_memory m (valid_references m) ->
+  (* --- *)
+  ad < #m ->
+  valid_references m t1 ->
+  t1 --[e_acq tid ad m[ad].t]--> t2 ->
+  valid_references m[ad.X <- X] t2.
+Proof.
+  intros.
+  ind_tstep; invc_vr; eauto using vr_mem_setX, valid_references.
+  repeat invc_vr; eauto using vr_subst, vr_mem_setX, valid_references.
+Qed.
+
+Lemma vr_preservation_unt_acq : forall m t1 t2 tu tid ad t X,
+  ad < #m ->
+  valid_references m tu ->
+  t1 --[e_acq tid ad t]--> t2 ->
+  valid_references m[ad.X <- X] tu.
+Proof.
+  eauto using vr_mem_setX.
+Qed.
 
 (* rel --------------------------------------------------------------------- *)
 
-Lemma vr_preservation_mem_rel : forall m1 m2 t1 t2 otid1 otid2 t tid ad,
-  forall_memory m1 well_typed_term ->
+Lemma vr_preservation_mem_rel : forall m t1 t2 tid ad X,
+  forall_memory m well_typed_term ->
   well_typed_term t1 ->
-  valid_references m1 t1 ->
-  (* --- *)
-  ad < #m1 ->
-  m1[ad].tm = <{ptm otid1 t}> ->
-  m2 = m1[ad <- (<{ptm otid2 t}>, m1[ad].ty)] ->
-  (* --- *)
-  forall_memory m1 (valid_references m1) ->
-  t1 --[e_rel tid ad]--> t2 ->
-  forall_memory m2 (valid_references m2).
-Proof.
-  intros.
-  ind_tstep; invc_wtt; invc_vr; eauto.
-  intros ?. Array.sgs.
-  - repeat clean; simpl.
-    eapply vr_ptm.
-    eapply vr_mem_setX'; trivial.
-    + admit.
-    + admit.
-    + admit.
-  - repeat clean.
-  (*
-  specialize (Hmvad ad'). simpl in *.
-  rewrite Hptm in Hmvad. invc Hmvad.
-  eauto using vad_mem_set, valid_addresses.
-  *)
-Abort.
-
-Lemma vad_preservation_rel : forall m t1 t2 otid1 otid2 t tid ad T,
-  forall_memory m (valid_addresses m) ->
+  valid_references m t1 ->
   (* --- *)
   ad < #m ->
-  m[ad].tm = <{ptm otid1 t}> ->
-  (* --- *)
-  valid_addresses m t1 ->
+  forall_memory m (valid_references m) ->
   t1 --[e_rel tid ad]--> t2 ->
-  valid_addresses m[ad <- (<{ptm otid2 t}>, T)] t2.
+  forall_memory m[ad.X <- X] (valid_references m[ad.X <- X]).
 Proof.
-  intros.
-  ind_tstep; inv_vad; eauto using vad_mem_set, valid_addresses.
+  intros ** ?. omicron; eauto using vr_mem_setX.
 Qed.
 
-Lemma vad_preservation_unt_rel : forall m t1 t2 tu otid1 otid2 t tid ad T,
-  forall_memory m (valid_addresses m) ->
-  (* --- *)
+Lemma vr_preservation_rel : forall m t1 t2 tid ad X,
   ad < #m ->
-  m[ad].tm = <{ptm otid1 t}> ->
-  (* --- *)
-  valid_addresses m tu ->
+  valid_references m t1 ->
   t1 --[e_rel tid ad]--> t2 ->
-  valid_addresses m[ad <- (<{ptm otid2 t}>, T)] tu.
+  valid_references m[ad.X <- X] t2.
 Proof.
-  eauto using vad_mem_set.
+  intros.
+  ind_tstep; invc_vr; eauto using vr_mem_setX, valid_references.
+Qed.
+
+Lemma vr_preservation_unt_rel : forall m t1 t2 tu tid ad X,
+  ad < #m ->
+  valid_references m tu ->
+  t1 --[e_rel tid ad]--> t2 ->
+  valid_references m[ad.X <- X] tu.
+Proof.
+  eauto using vr_mem_setX.
 Qed.
 
 (* spawn ------------------------------------------------------------------- *)
@@ -448,12 +404,12 @@ Proof.
   - eauto using vr_preservation_mem_write.
   - eauto using vr_preservation_write.
   - eauto using vr_preservation_unt_write.
-  - admit.
-  - admit.
-  - admit.
-  - admit.
-  - admit.
-  - admit.
+  - eauto using vr_preservation_mem_acq.
+  - eauto using vr_preservation_acq.
+  - eauto using vr_preservation_unt_acq.
+  - eauto using vr_preservation_mem_rel.
+  - eauto using vr_preservation_rel.
+  - eauto using vr_preservation_unt_rel.
   - eauto using vr_preservation_spawn.
   - eauto using vr_preservation_spawned.
   - eauto using valid_references.
@@ -477,6 +433,4 @@ Proof.
     by (eapply vr_preservation; eauto).
   destruct_forall_program. assumption.
 Qed.
-
-
 
